examples/sys_regs.v
@@ -1,22 +1,22 @@
 Require Import isla.base.
 Require Import isla.automation.
 
-Definition sys_regs : list (reg_col_entry * valu) := [
-  (RegColDirect "SCTLR_EL2" , Val_Bits [BV{64} 0x0000000004000002] );
-  (RegColDirect "SCR_EL3" , Val_Bits [BV{32} 0] );
-  (RegColDirect "TCR_EL2" , Val_Bits [BV{64} 0] );
-  (RegColDirect "CFG_ID_AA64PFR0_EL1_EL0" , Val_Bits [BV{4} 1] );
-  (RegColDirect "CFG_ID_AA64PFR0_EL1_EL1" , Val_Bits [BV{4} 1] );
-  (RegColDirect "CFG_ID_AA64PFR0_EL1_EL2" , Val_Bits [BV{4} 1] );
-  (RegColDirect "CFG_ID_AA64PFR0_EL1_EL3" , Val_Bits [BV{4} 1] );
-  (RegColDirect "OSLSR_EL1" , Val_Bits [BV{32} 0] );
-  (RegColDirect "OSDLR_EL1" , Val_Bits [BV{32} 0] );
-  (RegColDirect "EDSCR" , Val_Bits [BV{32} 0] );
-  (RegColDirect "MPIDR_EL1" , Val_Bits [BV{64} 0] );
-  (RegColStruct "PSTATE" "SP" , Val_Bits [BV{1} 1] );
-  (RegColStruct "PSTATE" "EL" , Val_Bits [BV{2} 2] );
-  (RegColStruct "PSTATE" "nRW" , Val_Bits [BV{1} 0] );
-  (RegColStruct "PSTATE" "D" , Val_Bits [BV{1} 1])
+Definition sys_regs : list (reg_col_entry * option valu) := [
+  (RegColDirect "SCTLR_EL2" , Some (Val_Bits [BV{64} 0x0000000004000002]) );
+  (RegColDirect "SCR_EL3" , Some (Val_Bits [BV{32} 0]) );
+  (RegColDirect "TCR_EL2" , Some (Val_Bits [BV{64} 0]) );
+  (RegColDirect "CFG_ID_AA64PFR0_EL1_EL0" , Some (Val_Bits [BV{4} 1]) );
+  (RegColDirect "CFG_ID_AA64PFR0_EL1_EL1" , Some (Val_Bits [BV{4} 1]) );
+  (RegColDirect "CFG_ID_AA64PFR0_EL1_EL2" , Some (Val_Bits [BV{4} 1]) );
+  (RegColDirect "CFG_ID_AA64PFR0_EL1_EL3" , Some (Val_Bits [BV{4} 1]) );
+  (RegColDirect "OSLSR_EL1" , Some (Val_Bits [BV{32} 0]) );
+  (RegColDirect "OSDLR_EL1" , Some (Val_Bits [BV{32} 0]) );
+  (RegColDirect "EDSCR" , Some (Val_Bits [BV{32} 0]) );
+  (RegColDirect "MPIDR_EL1" , Some (Val_Bits [BV{64} 0]) );
+  (RegColStruct "PSTATE" "SP" , Some (Val_Bits [BV{1} 1]) );
+  (RegColStruct "PSTATE" "EL" , Some (Val_Bits [BV{2} 2]) );
+  (RegColStruct "PSTATE" "nRW" , Some (Val_Bits [BV{1} 0]) );
+  (RegColStruct "PSTATE" "D" , Some (Val_Bits [BV{1} 1]))
 ].
 
 Definition sys_regs_map : reg_map :=
@@ -57,7 +57,7 @@ Section sys_regs.
     "PSTATE" # "V" ↦ᵣ Val_Bits [BV{1} 0] ∗
     "PSTATE" # "Z" ↦ᵣ Val_Bits [BV{1} 0].
   Proof.
-    rewrite /reg_col/=.
+    rewrite !reg_col_cons_Some reg_col_nil.
     repeat (rewrite big_sepM_insert;[ | by vm_compute]).
     iIntros "Hctx H". repeat iDestruct "H" as "[$ H]".
     iDestruct "H" as "[HPSTATE _]".
